[examples/lambda] Some minor tweaks to results about appstar
Use

  Induct_on `x` using SNOC_INDUCT

idiom more and also add some more rewrites.

examples/lambda/barendregt/chap2Script.sml
@@ -87,7 +87,9 @@ Inductive lameq :
      (!M N. M == N ==> N == M) /\
 [~TRANS:]
      (!M N L. M == N /\ N == L ==> M == L) /\
+[~APPL:]
      (!M N Z. M == N ==> M @@ Z == N @@ Z) /\
+[~APPR:]
      (!M N Z. M == N ==> Z @@ M == Z @@ N) /\
      (!M N x. M == N ==> LAM x M == LAM x N)
 End
@@ -343,8 +345,8 @@ val lameq_I = store_thm(
 Theorem I_appstar' :
     !Is. (!e. MEM e Is ==> e = I) ==> I @* Is == I
 Proof
-    HO_MATCH_MP_TAC SNOC_INDUCT >> rw []
- >> ASM_SIMP_TAC (betafy (srw_ss())) [SNOC_APPEND, SYM appstar_SNOC, lameq_I]
+  Induct_on ‘Is’ using SNOC_INDUCT >> rw [appstar_SNOC]
+  >> ASM_SIMP_TAC (betafy (srw_ss())) [lameq_I]
 QED
 
 Theorem I_appstar :
@@ -723,9 +725,7 @@ QED
 Theorem lameq_appstar_cong :
     !M N Ns. M == N ==> M @* Ns == N @* Ns
 Proof
-    NTAC 2 GEN_TAC
- >> HO_MATCH_MP_TAC SNOC_INDUCT >> rw []
- >> ASM_SIMP_TAC (betafy (srw_ss())) [SNOC_APPEND, SYM appstar_SNOC]
+  Induct_on ‘Ns’ using SNOC_INDUCT >> rw [appstar_SNOC, lameq_APPL]
 QED
 
 val _ = remove_ovl_mapping "Y" {Thy = "chap2", Name = "Y"}
